Veir/IR/GetSet.lean
@@ -1536,6 +1536,157 @@ theorem OpOperandPtrPtr.get!_OperationPtr_setRegions {opOperandPtr : OpOperandPt
     opOperandPtr.get! ctx := by
   grind
 
+
+/- OperationPtr.setRegions -/
+
+@[simp, grind =]
+theorem BlockPtr.get!_OperationPtr_pushRegion {block : BlockPtr} :
+    block.get! (OperationPtr.pushRegion operation' ctx newRegion hop') =
+    block.get! ctx := by
+  grind
+
+@[grind =]
+theorem OperationPtr.get!_OperationPtr_pushRegion {operation : OperationPtr} :
+    operation.get! (OperationPtr.pushRegion operation' ctx newRegion hop') =
+    if operation = operation' then
+      { operation.get! ctx with regions := (operation.get! ctx).regions.push newRegion }
+    else
+      operation.get! ctx := by
+  grind
+
+@[simp, grind =]
+theorem OperationPtr.prev!_OperationPtr_pushRegion {operation : OperationPtr} :
+    (operation.get! (OperationPtr.pushRegion operation' ctx newRegion hop')).prev =
+    (operation.get! ctx).prev := by
+  grind
+
+@[simp, grind =]
+theorem OperationPtr.next!_OperationPtr_pushRegion {operation : OperationPtr} :
+    (operation.get! (OperationPtr.pushRegion operation' ctx newRegion hop')).next =
+    (operation.get! ctx).next := by
+  grind
+
+@[simp, grind =]
+theorem OperationPtr.parent!_OperationPtr_pushRegion {operation : OperationPtr} :
+    (operation.get! (OperationPtr.pushRegion operation' ctx newRegion hop')).parent =
+    (operation.get! ctx).parent := by
+  grind
+
+@[simp, grind =]
+theorem OperationPtr.opType!_OperationPtr_pushRegion {operation : OperationPtr} :
+    (operation.get! (OperationPtr.pushRegion operation' ctx newRegion hop')).opType =
+    (operation.get! ctx).opType := by
+  grind
+
+@[simp, grind =]
+theorem OperationPtr.attrs!_OperationPtr_pushRegion {operation : OperationPtr} :
+    (operation.get! (OperationPtr.pushRegion operation' ctx newRegion hop')).attrs =
+    (operation.get! ctx).attrs := by
+  grind
+
+@[simp, grind =]
+theorem OperationPtr.properties!_OperationPtr_pushRegion {operation : OperationPtr} :
+    operation.getProperties! (OperationPtr.pushRegion operation' ctx newRegion hop') =
+    operation.getProperties! ctx := by
+  grind
+
+@[simp, grind =]
+theorem OperationPtr.getNumResults!_OperationPtr_pushRegion {operation : OperationPtr} :
+    operation.getNumResults! (OperationPtr.pushRegion operation' ctx hop' newRegion) =
+    operation.getNumResults! ctx := by
+  grind
+
+@[simp, grind =]
+theorem OpResultPtr.get!_OperationPtr_pushRegion {opResult : OpResultPtr} :
+    opResult.get! (OperationPtr.pushRegion operation' ctx newRegion hop') =
+    opResult.get! ctx := by
+  grind
+
+@[simp, grind =]
+theorem OperationPtr.getNumOperands!_OperationPtr_pushRegion {operation : OperationPtr} :
+    operation.getNumOperands! (OperationPtr.pushRegion operation' ctx hop' newRegion) =
+    operation.getNumOperands! ctx := by
+  grind
+
+@[simp, grind =]
+theorem OpOperandPtr.get!_OperationPtr_pushRegion {opOperand : OpOperandPtr} :
+    opOperand.get! (OperationPtr.pushRegion operation' ctx newRegion hop') =
+    opOperand.get! ctx := by
+  grind
+
+@[simp, grind =]
+theorem OperationPtr.getNumSuccessors!_OperationPtr_pushRegion {operation : OperationPtr} :
+    operation.getNumSuccessors! (OperationPtr.pushRegion operation' ctx newRegion hop') =
+    operation.getNumSuccessors! ctx := by
+  grind
+
+@[simp, grind =]
+theorem BlockOperandPtr.get!_OperationPtr_pushRegion {blockOperand : BlockOperandPtr} :
+    blockOperand.get! (OperationPtr.pushRegion operation' ctx newRegion hop') =
+    blockOperand.get! ctx := by
+  grind
+
+@[grind =]
+theorem OperationPtr.getNumRegions!_OperationPtr_pushRegion {operation : OperationPtr} :
+    operation.getNumRegions! (OperationPtr.pushRegion operation' ctx newRegion hop') =
+    if operation = operation' then
+      operation.getNumRegions! ctx + 1
+    else
+      operation.getNumRegions! ctx := by
+  grind
+
+@[grind =]
+theorem OperationPtr.getRegion!_OperationPtr_pushRegion {operation : OperationPtr} :
+    operation.getRegion! (OperationPtr.pushRegion operation' ctx newRegion hop') index =
+    if operation = operation' ∧ index = operation.getNumRegions! ctx then
+      newRegion
+    else
+      operation.getRegion! ctx index := by
+  grind
+
+@[simp, grind =]
+theorem BlockOperandPtrPtr.get!_OperationPtr_pushRegion {blockOperandPtr : BlockOperandPtrPtr} :
+    blockOperandPtr.get! (OperationPtr.pushRegion operation' ctx newRegion hop') =
+    blockOperandPtr.get! ctx := by
+  grind
+
+@[simp, grind =]
+theorem BlockPtr.getNumArguments!_OperationPtr_pushRegion {block : BlockPtr} {hop} :
+    block.getNumArguments! (OperationPtr.pushRegion op ctx newRegion hop) =
+    block.getNumArguments! ctx := by
+  grind
+
+@[simp, grind =]
+theorem BlockArgumentPtr.get!_OperationPtr_pushRegion {blockArg : BlockArgumentPtr} :
+    blockArg.get! (OperationPtr.pushRegion operation' ctx newRegion hop') =
+    blockArg.get! ctx := by
+  grind
+
+@[simp, grind =]
+theorem RegionPtr.get!_OperationPtr_pushRegion {region : RegionPtr} :
+    region.get! (OperationPtr.pushRegion operation' ctx newRegion hop') =
+    region.get! ctx := by
+  grind
+
+@[simp, grind =]
+theorem ValuePtr.getFirstUse!_OperationPtr_pushRegion {value : ValuePtr} :
+    value.getFirstUse! (OperationPtr.pushRegion operation' ctx newRegion hop') =
+    value.getFirstUse! ctx := by
+  grind
+
+@[simp, grind =]
+theorem ValuePtr.getType!_OperationPtr_pushRegion {value : ValuePtr} :
+    value.getType! (OperationPtr.pushRegion operation' ctx newRegion hop') =
+    value.getType! ctx := by
+  grind
+
+@[simp, grind =]
+theorem OpOperandPtrPtr.get!_OperationPtr_pushRegion {opOperandPtr : OpOperandPtrPtr} :
+    opOperandPtr.get! (OperationPtr.pushRegion operation' ctx newRegion hop') =
+    opOperandPtr.get! ctx := by
+  grind
+
+
 /- BlockArgumentPtr.setType -/
 
 @[grind =]
